Checkpoint

Lambda.lean
@@ -29,9 +29,6 @@ theorem noVarZero : Var zero → False := by
   apply x
   rfl
 
-
-
-
 inductive Term : Context → Type  
 | var : ∀ {Γ}, Var Γ → Term Γ 
 | lam : ∀ {Γ}, Term (succ Γ) → Term Γ
@@ -99,7 +96,7 @@ inductive Step : ∀{Γ}, Term Γ → Term Γ → Type where
     Step N N' → Step (lam N) (lam N')
 
 | eta : ∀{Γ} {N : Term Γ},
-    Step N (lam (app (rename Var.succ N) (var Var.zero)))
+    Step (lam (app (rename Var.succ N) (var Var.zero))) N
 
 -- infix:50 " ==> " => Step
 
@@ -293,7 +290,7 @@ theorem composeRename {n1} {M : Term n1}
 def ren' {ren : {Γ : Context} → Ren Γ (Nat.succ Γ)}
   : ∀{Γ}, Ren Γ (succ Γ) := fun {Γ} => match Γ with
   | Nat.zero => fun y => False.rec (noVarZero y)
-  | Nat.succ x' => ext ren
+  | Nat.succ _x' => ext ren
 
 theorem commuteSubstRename {Γ} {M : Term Γ}
   : ∀ {Δ} {sub : Subst Γ Δ}
@@ -371,14 +368,6 @@ theorem subAssoc {n1 n2 n3 n4} {sub1 : Subst n1 n2} {sub2 : Subst n2 n3}
   simp [compose]
   apply subSub
 
-#check substZConsIds
-#check extsConsShift
-#check subDist
-#check subAssoc
-#check subIdR
-#check subIdL
-#check substZConsIds
-
 theorem subTail {n1 n2} {M : Term n2} {sub : Subst n1 n2}
   : compose shift (cons M sub) = sub := by
   apply funext
@@ -425,411 +414,229 @@ theorem renameSubstCommute {Γ Δ} {N : Term (succ Γ)} {M : Term Γ} {ren : Ren
 --------------------------------------------------------------------------------
 ---------- This section came from Confluence.agda in plfa ----------------------
 --------------------------------------------------------------------------------
--- I have heavily modified this section from PLFA
+-- I have modified this section from PLFA to handle eta
 
-def SubStep {n1 n2 : Context} (sub1 sub2 : Subst n1 n2) : Type :=
-  ∀ {x}, Step (sub1 x) (sub2 x)
+inductive Par : ∀{Γ}, Term Γ → Term Γ → Type   
+| pvar : ∀{Γ} {x : Var Γ}, Par (var x) (var x)
+| plam : ∀{Γ} {N N' : Term (succ Γ)},
+  Par N N' → Par (lam N) (lam N')  
+| papp : ∀{Γ}{L L' M M' : Term Γ},
+  Par L L' → Par M M' → Par (app L M) (app L' M')   
+| pbeta : ∀{Γ}{N N' : Term (succ Γ)} {M M' : Term Γ},
+  Par N N' → Par M M' → Par (app (lam N) M) (subLast N' M')  
+| peta : ∀{Γ} {M M' : Term Γ},
+  Par M M'
+  → Par (lam (app (rename Var.succ M) (var Var.zero))) M'
 
-def MultiSubStep {n1 n2} (sub1 sub2 : Subst n1 n2) : Type :=
-  ∀ {x}, MultiStep (sub1 x) (sub2 x)
+theorem subPar {Γ} {N N' : Term (succ Γ)} { M M' : Term Γ}
+  (p1 : Par N N') (p2 : Par M M')
+  : Par (subLast N M) (subLast N' M') := by
+  sorry
 
-def singletonStep {n} {t1 t2 : Term n} (step : Step t1 t2)
-  : MultiStep t1 t2 := MultiStep.step step MultiStep.halt
+theorem parRefl {Γ} {M : Term Γ} : Par M M := by
+  induction M with
+  | var i => apply Par.pvar
+  | app t1 t2 ih1 ih2 => apply Par.papp; apply ih1; apply ih2
+  | lam t ih => apply Par.plam; apply ih
 
-theorem multiSubStepHalt {n1 n2} {sub : Subst n1 n2} : MultiSubStep sub sub := by
-  intro x
-  apply MultiStep.halt
+inductive MultiPar {Γ} : Term Γ → Term Γ → Type  
+| halt : {M : Term Γ} → MultiPar M M 
+| step : {L M N : Term Γ}
+  → Par L M → MultiPar M N → MultiPar L N   
 
-theorem multiSubStepStep {n1 n2} {sub1 sub2 sub3 : Subst n1 n2}
-  (step : SubStep sub1 sub2) (mstep : MultiSubStep sub2 sub3)
-  : MultiSubStep sub1 sub3 := by
-  intro x
-  apply MultiStep.step step mstep
-
-theorem renameStep {n1}
-  {t1 t2 : Term n1} (step : Step t1 t2)
-  : ∀ {n2} {ren : Ren n1 n2},
-    Step (rename ren t1) (rename ren t2) := by 
-  induction step with
-  -- . simp [rename]; apply Step.app1;  
-  | app1 _ ih => intros; simp [rename]; apply Step.app1; apply ih
-  | app2 _ ih => intros; simp [rename]; apply Step.app2; apply ih
-  | lam _ ih => intros; simp [rename]; apply Step.lam; apply ih
-  | beta =>
-    intros
-    simp [rename]
-    rw [<- renameSubstCommute]
-    apply Step.beta
-  | eta =>
-    intros
-    simp [rename]
-    rw [composeRename]
-    -- TODO: decide if this lemma should be defined outside. Is it needed elsewhere?
-    have renExtLemma : ∀{n1 n2} {ren : Ren n1 n2}, ext ren ∘ Var.succ = Var.succ ∘ ren := by
-      intros
-      apply funext
-      intro x
-      simp [Function.comp]
-      simp [ext]
-    rw [renExtLemma]
-    rw [<- composeRename]
-    apply Step.eta
-
-theorem renameMultiStep {n1}
-  {t1 t2 : Term n1} {mstep : MultiStep t1 t2}
-  : ∀ {n2} {ren : Ren n1 n2},
-    MultiStep (rename ren t1) (rename ren t2) := by 
-  induction mstep with
-  | halt => intros; apply MultiStep.halt
-  | step s _ms ih =>
-    intros
-    apply MultiStep.step
-    apply (renameStep s)
-    apply ih
-  
-
-theorem subStepExts {n1 n2} {sub1 sub2 : Subst n1 n2}
-  : SubStep sub1 sub2 → MultiSubStep (exts sub1) (exts sub2) := by 
-  intro step x
-  cases x with
-  | zero => simp [exts]; apply MultiStep.halt
-  | succ y => simp [exts]; apply renameMultiStep; apply singletonStep; apply step
-
-theorem subMultiStepExts {n1 n2} {sub1 sub2 : Subst n1 n2}
-  : MultiSubStep sub1 sub2 → MultiSubStep (exts sub1) (exts sub2) := by 
-  intro mstep x
-  cases x with
-  | zero => simp [exts]; apply multiSubStepHalt
-  | succ y =>
-    simp [exts]
-    apply renameMultiStep
-    apply mstep
-
-
-theorem substStep {n1}
-  {t1 t2 : Term n1} (step : Step t1 t2)
-  : ∀ {n2} {sub : Subst n1 n2},
-    Step (subst sub t1) (subst sub t2) := by 
-  induction step with
-  | app1 _ ih => intros; simp [subst]; apply Step.app1; apply ih
-  | app2 _ ih => intros; simp [subst]; apply Step.app2; apply ih
-  | lam _ ih => intros; simp [subst]; apply Step.lam; apply ih
-  | beta =>
-    intros
-    simp [subst]
-    rw [<- substCommute]
-    apply Step.beta
-  | @eta _ N =>
-    intros n2 sub
-    simp [subst]
-    have lemma : subst (exts sub) (rename Var.succ N) = rename Var.succ (subst sub N) := by
-      rw [renameSubstRen]
-      rw [renameSubstRen]
-      rw [subSub]
-      rw [subSub]
-      rw [renSuccShift]
-      rw [renSuccShift]
-      rw [extsConsShift]
-      rw [subTail]
-    rw [lemma]
-    apply Step.eta
-
-theorem substMultiStep {n1}
-  {t1 t2 : Term n1} (step : MultiStep t1 t2)
-  {n2} {sub : Subst n1 n2}
-  : MultiStep (subst sub t1) (subst sub t2) := by 
-  induction step with
-  | halt => apply MultiStep.halt
-  | step s ms ih =>
-    apply MultiStep.step
-    apply (substStep s)
-    apply ih
-  
-  
-theorem stepSubs {n1} {t : Term n1} :
-   ∀ {n2} {sub1 sub2 : Subst n1 n2} {_sstep : MultiSubStep sub1 sub2},
-    MultiStep (subst sub1 t) (subst sub2 t) := by
-  induction t with
-  | var x => intro n2 sub1 sub2 sstep; apply sstep
-  | app t1 t2 ih1 ih2 =>
-    intro n2 sub1 sub2 sstep
-    simp [subst]
-    apply appCong
-    apply ih1; apply sstep
-    apply ih2; apply sstep
-  | lam t ih =>
-    intro n2 sub1 sub2 sstep
-    simp [subst]
-    apply lamCong
-    apply ih
-    apply subMultiStepExts
-    apply sstep
-  
-theorem parSubstZero {Γ} {M M' : Term Γ}
-   {mstep: MultiStep M M' }
-   : MultiSubStep (substZero M) (substZero M') := by
-   intro x
-   cases x
-   . apply mstep
-   . simp [substZero]
-     apply MultiStep.halt
-
-theorem stepSub {Γ} {N N' : Term (succ Γ)} {M M' : Term Γ}
-  (stepN : MultiStep N N') (stepM : MultiStep M M')
-  : MultiStep (subLast N M) (subLast N' M') := by
-  simp [subLast]
-  let lemma : MultiStep (subst (substZero M) N) (subst (substZero M) N') := by
-      apply substMultiStep
-      apply stepN
-  apply (multiTrans lemma)
-  apply stepSubs
-  apply parSubstZero
-  apply stepM
-
-def superStep {Γ} (t : Term Γ) : Term Γ :=
+-- Σ' is called "psigma"
+-- would need to generalize so that induction works in lambda case
+def unweaken {Γ} (t : Term (succ Γ))
+  : Option (Σ' t', rename Var.succ t' = t) :=
+  -- should actually be (does not exists t' such that ...) ⊕ (Σ' t', rename Var.succ t' = t)
   match t with
-  | var x => var x
-  | app (lam t1) t2 => subLast (superStep t1) (superStep t2)
-  | app t1 t2 => app (superStep t1) (superStep t2)
-  | lam t => lam (superStep t)
+  | var i => match i with
+    | Var.zero => none
+    | Var.succ i' => some ⟨var i', rfl⟩
+  | app t1 t2 => do
+    let ⟨t1', p1⟩ <- unweaken t1
+    let ⟨t2', p2⟩  <- unweaken t2
+    some ⟨app t1' t2', by simp [rename]; apply And.intro; apply p1; apply p2⟩ 
+  | lam t => do
+    let ⟨t', p⟩ <- unweaken t
+    some ⟨lam t', by simp [rename]; apply p⟩ 
 
-inductive BetaStep : ∀{Γ}, Term Γ → Term Γ → Type where  
-| app1 : ∀ {Γ} {L L' M : Term Γ},
-    BetaStep L L'
-    → BetaStep (app L M) (app L' M)
-| app2 : ∀ {Γ} {L M M' : Term Γ},
-    BetaStep M M'
-    → BetaStep (app L M) (app L M')
-| beta : ∀ {Γ} {N : Term (succ Γ)} {M : Term Γ},
-    BetaStep (app (lam N) M) (subLast N M)
-| lam : ∀ {Γ} {N N' : Term (succ Γ)},
-    BetaStep N N' → BetaStep (lam N) (lam N')
+inductive PropToType (P : Prop) : Type
+| propToType : P → PropToType P
 
-inductive EtaStep : ∀{Γ}, Term Γ → Term Γ → Type where  
-| eta : ∀{Γ} {N : Term Γ},
-    EtaStep N (lam (app (rename Var.succ N) (var Var.zero)))
+-- see also: https://www.cs.vu.nl/~jbe248/lv2017/12x4.pdf
+-- see https://doi.org/10.1006/inco.1995.1057
+-- universal common reduct
+-- def ucr {Γ} (t : Term Γ) : Term Γ :=
+--   match t with
+--   | var x => var x
+--   | app (lam t1) t2 => subLast (ucr t1) (ucr t2)
+--   | lam term@(app t (var Var.zero)) =>
+--     match unrename Var.succ t with
+--     | Sum.inl _ => lam (ucr term)
+--     | Sum.inr ⟨t', _p⟩ => t'
+--   | lam (var i) => lam (ucr (var i))
+--   -- | lam (lam t) => lam (ucr (lam t))
+--   | lam t => lam (ucr t)
+--   | app t1 t2 => app (ucr t1) (ucr t2)
 
-theorem selfSuperStep {Γ} {t : Term Γ}
-  : MultiStep t (superStep t) :=
+inductive Decided (P : Prop) : Type
+| yes : P → Decided P 
+| no : Not P → Decided P 
+
+inductive DecidedT (T : Type) : Type
+| yes : T → DecidedT T 
+| no : (T → False) → DecidedT T 
+
+-- TODO: is it called a redEx?
+inductive BetaRedux {Γ} : Term Γ → Prop
+| redux : ∀ {t1 t2}, BetaRedux (app (lam t1) t2)
+
+inductive EtaRedux : ∀{Γ}, Term Γ → Prop
+| redux : ∀ {t}, EtaRedux (lam (app (rename Var.succ t) (var Var.zero)))
+
+inductive TermKind : ∀{Γ}, Term Γ → Type
+| betaRedux : ∀{Γ}, (t1 : Term (succ Γ)) → (t2 : Term Γ)
+  →  TermKind (app (lam t1) t2)
+| app : ∀{Γ}, (t1 t2 : Term Γ) → Not (BetaRedux (app t1 t2)) 
+  → TermKind (app t1 t2) 
+| etaRedux : ∀{Γ}, (t : Term Γ)
+  → TermKind (lam (app (rename Var.succ t) (var Var.zero))) 
+| lam : ∀{Γ}, (t : Term (succ Γ)) → Not (EtaRedux (lam t))
+  → TermKind (lam t)
+| var : ∀{Γ}, (i : Var Γ) → TermKind (var i)
+
+def test {n} (t : Term (succ n)) : Term (succ n) :=
   match t with
-  | var i => by simp [superStep]; apply MultiStep.halt
-  | app (lam t1) t2 => by
-    simp [superStep]
-    apply MultiStep.step
-    apply Step.beta
-    apply stepSub
-    apply selfSuperStep
-    apply selfSuperStep
-  | app (app t1 t2) t3 => by
-    simp [superStep]
-    apply appCong
-    apply selfSuperStep
-    apply selfSuperStep
-  | app (var i) t2 => by
-    simp [superStep]
-    apply appCong
-    apply MultiStep.halt
-    apply selfSuperStep
-    --
-  | lam t => by
-    simp [superStep]
-    apply lamCong
-    apply selfSuperStep
+  | var _ => _
+  | lam _ => _
+  | app _ _ => _
 
-theorem triangleProperty {Γ} {t t' : Term Γ}
-  {step : BetaStep t t'}
-  : MultiStep t' (superStep t) :=
-  match t, t', step with
-  | .(_), .(_), BetaStep.lam s => by
-    simp [superStep]
-    apply lamCong
-    apply triangleProperty
-    apply s
-  | (app (var i) t2), .(_), BetaStep.app2 s => by
-    simp [superStep]
-    apply appRCong
-    apply triangleProperty
-    apply s
-  | (app (lam t1) t2), .(_), BetaStep.app2 s => by
-    simp [superStep]
-    apply MultiStep.step
-    apply Step.beta
-    apply stepSub
-    apply selfSuperStep
-    apply triangleProperty; apply s
-  | (app (app t1 t2) t3), .(_), BetaStep.app2 s => by
-    simp [superStep]
-    apply appCong
-    apply selfSuperStep
-    apply triangleProperty; apply s
-  | .(_), .(_), BetaStep.beta => by
-    simp [superStep]
-    apply stepSub
-    apply selfSuperStep
-    apply selfSuperStep
-  | (app (lam t1) t2), .(_), BetaStep.app1 (BetaStep.lam s) => by
-    simp [superStep]
-    apply MultiStep.step
-    apply Step.beta
-    apply stepSub
-    apply triangleProperty; apply s
-    apply selfSuperStep
-  | (app (app t1 t2) t3), .(_), BetaStep.app1 s => by
-    simp [superStep]
-    apply appCong
-    apply triangleProperty; apply s
-    apply selfSuperStep
+def unrename {n1 n2} (ren : Ren n1 n2) (t : Term n2)
+  : DecidedT (Σ' t', rename ren t' = t) :=
+  by sorry
 
-theorem betaToStep {n} {t1 t2 : Term n}
-  {bstep : BetaStep t1 t2} : Step t1 t2 := by
-  induction bstep with
-  | app1 _ ih => apply Step.app1; apply ih
-  | app2 _ ih => apply Step.app2; apply ih
-  | lam _ ih => apply Step.lam; apply ih
-  | beta => apply Step.beta
+theorem findTermKind {Γ : Context} (t : Term Γ) : TermKind t :=
+  match t with
+  | (app (lam t1) t2) => TermKind.betaRedux _ _
+  | (app (var _) t2) => TermKind.app _ _ (by intro r; cases r)
+  | (app (app _ _) t2) => TermKind.app _ _ (by intro r; cases r)
+  | (Term.lam t) =>
+    let whatIsWrongWithLean {n} (t : Term (succ n)) : TermKind (lam t) :=
+      match t with
+      | var _ => TermKind.lam _ (by intro r; cases r)
+      | lam _ => TermKind.lam _ (by intro r; cases r)
+      | app t1 (var (Var.succ _)) => TermKind.lam _ (by intro r; cases r)
+      | app t1 (app _ _) => TermKind.lam _ (by intro r; cases r)
+      | app t1 (lam _) => TermKind.lam _ (by intro r; cases r)
+      | app t1 (var Var.zero) => match unrename Var.succ t1 with
+        | DecidedT.yes ⟨t', p⟩ => by
+          rw [<- p]
+          exact TermKind.etaRedux _
+        | DecidedT.no p => TermKind.lam _ (by
+          intro x
+          cases x with
+          | @redux t =>
+            apply p
+            exists t
+        )
+    whatIsWrongWithLean t
+  | (var _) => TermKind.var _
 
--- theorem stepToBeta {n} {t1 t2 : Term n}
---   {step : Step t1 t2}
---   : BetaStep t1 t2 ⊕ EtaStep t1 t2 := by
---   induction step with
---   | app1 _ ih => apply Sum.inl; apply BetaStep.app1; apply ih
---   | app2 _ ih => apply Sum.inl; apply BetaStep.app2; apply ih
---   | lam _ ih => apply Sum.inl; apply BetaStep.lam; apply ih
---   | beta => apply Sum.inl; apply BetaStep.beta
---   | eta => apply Sum.inr; apply EtaStep.eta
+theorem decideBetaRedux {Γ} (t : Term Γ) : Decided (BetaRedux t) :=
+  match t with
+  | (app (lam t1) t2) => Decided.yes BetaRedux.redux
+  | (app (var _) t2) => Decided.no (by intro r; cases r)
+  | (app (app _ _) t2) => Decided.no (by intro r; cases r)
+  | (lam _) => Decided.no (by intro r; cases r)
+  | (var _) => Decided.no (by intro r; cases r)
 
-theorem subWeaken {n} {M N : Term n}
-  : subLast (rename Var.succ M) N = M := by
-  simp [subLast]
-  rw [renameSubstRen]
-  rw [subSub]
-  have lemma: compose (renToSub Var.succ) (substZero N) = ids := by
-    apply funext
-    intro x
-    cases x
-    . rfl
-    . rfl
-  rw [lemma]
-  apply subId
+inductive Ucr : ∀{Γ}, Term Γ → Term Γ → Type
+| var : ∀{i}, Ucr (var i) (var i)
+| beta : ∀{Γ}, {M M': Term (succ Γ)} → {N N' : Term Γ}  → Ucr M M' → Ucr N N' 
+  → Ucr (app (lam M) N) (subLast M' N') 
+| eta : ∀{Γ}, {M : Term Γ}
+  → Ucr (lam (app (rename Var.succ M) (var Var.zero))) M 
+| app : ∀{Γ}, {M N M' N' : Term Γ} → Not (BetaRedux (app M N)) 
+  → Ucr M M' → Ucr N N' → Ucr (app M N) (app M' N')  
+| lam : ∀{Γ}, {M M' : Term (succ Γ)} → Not (EtaRedux (lam M)) 
+  → Ucr M M' → Ucr (lam M) (lam M')
 
-theorem betaEtaCaseLemma {Γ} {M : Term Γ} {N : Term (succ Γ)}
-  : MultiStep (app (lam (app (rename Var.succ (lam N)) (var Var.zero))) M) (subLast N M)
-  := by
-     apply MultiStep.step
-     apply Step.beta
-     have lemma {n} {a : Term (succ n)} {M : Term n}
-       : subLast (app (rename Var.succ (lam a)) (var Var.zero)) M
-       = app (lam a) M := by
-       have lemma2 {n} {a : Term (succ n)} {M : Term n} 
-         : subLast (app (rename Var.succ (lam a)) (var Var.zero)) M
-           = app (subLast (rename Var.succ (lam a)) M) M := by
-           simp [subLast, subst, substZero]
-       rw [lemma2]
-       rw [subWeaken]
-     rw [lemma]
-     apply MultiStep.step
-     apply Step.beta
-     apply MultiStep.halt
+theorem ucrExists {Γ} (t : Term Γ) : Σ' t', Ucr t t' :=
+  match findTermKind t with
+  | TermKind.betaRedux t1 t2 => _
+  | TermKind.app t1 t2 p =>
+    match ucrExists t1, ucrExists t2 with
+    | ⟨t1', p1⟩, ⟨t2', p2⟩ => ⟨app t1' t2', Ucr.app p p1 p2⟩
+  | TermKind.lam t p => _
+  | TermKind.etaRedux t => _
+  | TermKind.var i => _
 
-theorem singleStepConfluence {Γ} {t t1 t2 : Term Γ}
-  (step1 : Step t t1) (step2 : Step t t2)
-  : Σ t', MultiStep t1 t' × MultiStep t2 t' :=
-  match step1, step2 with
-  | Step.lam a, Step.lam b => match singleStepConfluence a b with
-    | ⟨t, m1, m2⟩ => ⟨lam t, lamCong m1, lamCong m2⟩
-  | Step.app1 a, Step.app1 b => match singleStepConfluence a b with
-    | ⟨_, m1, m2⟩ => ⟨_, appLCong m1, appLCong m2⟩
-  | Step.app2 a, Step.app2 b => match singleStepConfluence a b with
-    | ⟨_, m1, m2⟩ => ⟨_, appRCong m1, appRCong m2⟩
-  | Step.app2 a, Step.app1 b => 
-    ⟨_, singletonStep (Step.app1 b), singletonStep (Step.app2 a)⟩
-  | Step.app1 a, Step.app2 b =>
-    ⟨_, singletonStep (Step.app2 b), singletonStep (Step.app1 a)⟩
-  | Step.eta, x => ⟨_,
-        singletonStep (Step.lam (Step.app1 (renameStep x)))
-        , singletonStep Step.eta⟩
-  | x, Step.eta => ⟨_,
-        singletonStep Step.eta
-        , singletonStep (Step.lam (Step.app1 (renameStep x)))⟩ 
-  | Step.beta, Step.beta => ⟨_, MultiStep.halt, MultiStep.halt⟩
-  | Step.beta, Step.app1 (Step.lam s) => ⟨_, stepSub (singletonStep s) MultiStep.halt,
-    singletonStep Step.beta⟩
-  | Step.beta, Step.app1 (Step.eta) => ⟨_, MultiStep.halt, betaEtaCaseLemma⟩
-  | Step.beta, Step.app2 a =>
-    ⟨_, stepSub MultiStep.halt (singletonStep a), singletonStep Step.beta⟩ 
-  | Step.app2 a, Step.beta =>
-    ⟨_, singletonStep Step.beta, stepSub MultiStep.halt (singletonStep a)⟩ 
-  | Step.app1 (Step.lam s), Step.beta => ⟨_, singletonStep Step.beta,
-    stepSub (singletonStep s) MultiStep.halt⟩
-  | Step.app1 Step.eta, Step.beta => ⟨_, betaEtaCaseLemma, MultiStep.halt⟩
+theorem parTriangle {Γ} {M N : Term Γ} (step: Par M N) : Par N (ucr M) :=
+  match M, step with
+  | .(_), Par.pvar => by simp [ucr]; apply parRefl
+  | .(_), Par.pbeta p1 p2 => by
+    simp [ucr]
+    apply subPar
+    apply parTriangle; apply p1
+    apply parTriangle; apply p2
+  | .(_), Par.peta p =>
+    let bla := parTriangle p
+    _ -- parTriangle p
+  | .(_), Par.papp Par.pvar p2 => by
+    simp [ucr]
+    apply Par.papp
+    apply parRefl
+    apply parTriangle; apply p2
+  | (app (lam t1) t2), Par.papp p1 p2 => _
+  | (app (app t1 t2) t3), Par.papp p1 p2 => _
+  | .(_), Par.plam p => _
 
-theorem strip {Γ} {t t1 t2 : Term Γ}
-  (step1 : Step t t1) (mstep2 : MultiStep t t2)
-  : Σ t', MultiStep t1 t' × MultiStep t2 t' :=
-  match mstep2 with
-  | MultiStep.halt => ⟨_, MultiStep.halt, singletonStep step1⟩
-  | MultiStep.step s ms =>
-    let bla := singleStepConfluence step1 s
-    match strip step1 mstep2 with
-    | ⟨t', ms1, ms2⟩ => ⟨_, _⟩
+def expand {Γ} (t : Term Γ) : Term Γ :=
+  lam (app (rename Var.succ t) (var Var.zero))
 
--- theorem confluence {Γ} {t t1 t2 : Term Γ}
---   (mstep1 : MultiStep t t1) (mstep2 : MultiStep t t2)
---   : Σ t', MultiStep t1 t' × MultiStep t2 t' := by
---   induction mstep1 with
---   | halt => exact ⟨_, mstep2, MultiStep.halt⟩
---   | step s1 ms1 ih1 => induction mstep2 with
---             | halt => exact ⟨_, MultiStep.halt, MultiStep.step s1 ms1⟩
---             | step s2 ms2 ih2 => sorry
+def ucr2 {Γ} (t : Term Γ) : Term Γ :=
+  expand (match t with
+          | var x => var x
+          | app (lam t1) t2 => subLast (ucr t1) (ucr t2)
+          | lam t => lam (ucr t)
+          | app t1 t2 => app (ucr t1) (ucr t2))
 
+inductive Par2 : ∀{Γ}, Term Γ → Term Γ → Type   
+| pvar : ∀{Γ} {x : Var Γ}, Par2 (var x) (var x)
+| plam : ∀{Γ} {N N' : Term (succ Γ)},
+  Par2 N N' → Par2 (lam N) (lam N')  
+| papp : ∀{Γ}{L L' M M' : Term Γ},
+  Par2 L L' → Par2 M M' → Par2 (app L M) (app L' M')   
+| pbeta : ∀{Γ}{N N' : Term (succ Γ)} {M M' : Term Γ},
+  Par2 N N' → Par2 M M' → Par2 (app (lam N) M) (subLast N' M')  
+-- | peta : ∀{Γ} {M M' : Term Γ},
+--   Par2 M M'
+--   → Par2 M (lam (app (rename Var.succ M') (var Var.zero)))
+| peta : ∀{Γ} {M M' : Term Γ},
+  Par2 (lam (app (rename Var.succ M) (var Var.zero))) M'
+  → Par2 M M' 
 
--- TODO: follow this proof https://doi.org/10.1006/inco.1995.1057
+theorem par2Refl {Γ} {M : Term Γ} : Par2 M M := by
+  induction M with
+  | var i => apply Par2.pvar
+  | app t1 t2 ih1 ih2 => apply Par2.papp; apply ih1; apply ih2
+  | lam t ih => apply Par2.plam; apply ih
 
-/- 
-Something that we will need
-Equivalence relation on terms R
+theorem renamePar2 {n1}
+  {t1 t2 : Term n1} (step : Par2 t1 t2)
+  : ∀ {n2} (ren : Ren n1 n2),
+    Par2 (rename ren t1) (rename ren t2) := by sorry
 
-lamR : R t1 t2 → R (lam t1) (lam t2)
-appR : R a1 a2 → R b1 b2 → R (app a1 b1) (app a2 b2)
-
-prove using *cong
----/
-
-
--- Something that is slightly concerning is if the use of funext and/or quotients
--- will make things non-computational in a way what will cause problems.
--- I need to think this through carefully.
-
--- I believe that the following demonstrates that quotients don't actually
--- get in the way of computation in lean:
-
-def Bla := @Quot Nat (fun x y => x = y)
-
-def getNat : Bla → Nat :=
-  Quot.lift (fun x => x) (by
-    intros a b p
-    simp
-    assumption
-  )
-
-theorem canICompute : (getNat (Quot.mk (fun x y => x = y) 5)) = 5 := by
-  simp
-
--- Some other very strange reduction behaviour that I noticed: any type with
--- only one constructor won't block reduction, but if you uncomment
--- the second constructor, then it does block reduction.
-
-inductive MyUnit : Type 
-| myunit : MyUnit
--- | myunit2 : MyUnit
-
-def test3 : MyUnit → Nat → Nat := fun p n =>
-  match p with
-  | MyUnit.myunit => n * n + 2
-  -- | MyUnit.myunit2 => n * n + 2
-
-axiom typeAxiom : MyUnit
-
-theorem canICompute2 : test3 typeAxiom 2 = 6 := by
-  simp [test3]
-  --
+theorem parTriangle2 {Γ} {M N : Term Γ} (step: Par2 M N) : Par2 N (ucr2 M) :=
+  match step with
+  | Par2.pvar => Par2.peta par2Refl
+  | Par2.pbeta p1 p2 => _
+  | Par2.peta p =>
+    let bla := parTriangle2 p
+    -- Par2.plam (Par2.papp (renamePar2 _ Var.succ) par2Refl) -- parTriangle p
+    _
+  | Par2.papp Par2.pvar p2 => _
+  | Par2.papp (Par2.plam p) p2 => _
+  | Par2.papp p1 p2 => _
+  | Par2.plam p => _
