LambdaOld.lean
@@ -1,0 +1,835 @@
+-- This file is a translation of PLFA
+
+-- https://leanprover.github.io/theorem_proving_in_lean4/inductive_types.html
+
+--------------------------------------------------------------------------------
+---------- This section came from Untyped.agda in plfa -------------------------
+--------------------------------------------------------------------------------
+
+
+open Nat
+open Fin
+open Option
+
+def Context : Type := Nat
+-- def Var : Context → Type := Fin
+
+inductive Var : Context → Type 
+| zero : ∀ {Γ}, Var (succ Γ)
+| succ : ∀ {Γ}, Var Γ → Var (succ Γ) 
+
+theorem noVarZero : Var zero → False := by
+  let gen : (∀{n}, Var n → n = zero → False) := by
+    intro n x
+    induction x with
+    | zero => simp
+    | succ _ =>  simp
+  intro x
+  apply gen
+  apply x
+  rfl
+
+
+
+
+inductive Term : Context → Type  
+| var : ∀ {Γ}, Var Γ → Term Γ 
+| lam : ∀ {Γ}, Term (succ Γ) → Term Γ
+| app : ∀ {Γ}, Term Γ → Term Γ → Term Γ  
+
+open Term
+
+def Ren (n1 n2 : Context) : Type := Var n1 → Var n2 
+
+def ext {n1 n2} (ren1 : Ren n1 n2) : (Ren (succ n1) (succ n2))
+  := fun x => match x with
+              | Var.zero => Var.zero
+              | Var.succ x' => Var.succ (ren1 x')
+
+def rename {n1 n2} (ren : Ren n1 n2) (t : Term n1) : Term n2 :=
+  match t with
+  | var i => var (ren i)
+  | lam t => lam (rename (ext ren) t)
+  | app t1 t2 => app (rename ren t1) (rename ren t2)
+
+def Subst (n1 n2 : Context) : Type := Var n1 → Term n2 
+
+def exts {n1 n2} (sub : Subst n1 n2) : Subst (succ n1) (succ n2) :=
+  fun x => match x with
+           | Var.zero => var Var.zero
+           | Var.succ x' => rename Var.succ (sub x')
+
+def subst {n1 n2} (sub : Subst n1 n2) (t : Term n1) : Term n2 :=
+  match t with
+  | var i => sub i
+  | lam t => lam (subst (exts sub) t)
+  | app t1 t2 => app (subst sub t1) (subst sub t2)
+
+def substZero {Γ} (t : Term Γ) : Subst (succ Γ) Γ :=
+  fun x => match x with
+           | Var.zero => t
+           | Var.succ x' => var x'
+
+def subLast {n} (t1 : Term (succ n)) (t2 : Term n) : Term n :=
+  subst (substZero t2) t1
+
+mutual
+  inductive Neutral : ∀{Γ}, Term Γ → Type  
+  | var : ∀{Γ}, (x : Var Γ) → Neutral (var x) 
+  | app : ∀{Γ}, {t1 t2 : Term Γ} → Neutral t1 → Normal t2 → Neutral (app t1 t2) 
+
+  inductive Normal : ∀{Γ}, Term Γ → Type  
+  | neu : ∀{Γ}, {t : Term Γ} → Neutral t → Normal t 
+  | lam : ∀{Γ}, {t : Term (succ Γ)} → Normal t → Normal (lam t) 
+end
+
+inductive Step : ∀{Γ}, Term Γ → Term Γ → Type where  
+| app1 : ∀ {Γ} {L L' M : Term Γ},
+    Step L L'
+    → Step (app L M) (app L' M)
+
+| app2 : ∀ {Γ} {L M M' : Term Γ},
+    Step M M'
+    → Step (app L M) (app L M')
+
+| beta : ∀ {Γ} {N : Term (succ Γ)} {M : Term Γ},
+    Step (app (lam N) M) (subLast N M)
+
+| lam : ∀ {Γ} {N N' : Term (succ Γ)},
+    Step N N' → Step (lam N) (lam N')
+
+| eta : ∀{Γ} {N : Term Γ},
+    Step N (lam (app (rename Var.succ N) (var Var.zero)))
+
+-- infix:50 " ==> " => Step
+
+inductive MultiStep : ∀ {Γ}, Term Γ → Term Γ → Type
+| halt : ∀ {Γ} {t : Term Γ}, MultiStep t t
+| step : ∀ {Γ} {t1 t2 t3 : Term Γ},
+  Step t1 t2 → MultiStep t2 t3 → MultiStep t1 t3  
+
+def progress {Γ} (M : Term Γ)
+  : (Σ N, Step M N) ⊕ (Normal M)
+  := match M with
+     | (var x) => Sum.inr (Normal.neu (Neutral.var x))
+     | lam N => match progress N with
+                | Sum.inl ⟨_ , s⟩ => Sum.inl ⟨_ , Step.lam s⟩ 
+                | Sum.inr t => Sum.inr (Normal.lam t)
+     | (app (lam _) _) => Sum.inl ⟨_ , Step.beta⟩
+     | (app (var x) M) => match progress M with
+              | Sum.inl ⟨_ , s⟩ => Sum.inl ⟨_ , Step.app2 s⟩
+              | Sum.inr normN => Sum.inr (Normal.neu (Neutral.app (Neutral.var x) normN))
+     | (app (app a b) M) => match progress (app a b) with
+              | Sum.inl ⟨_ , s⟩ => Sum.inl ⟨_ , Step.app1 s⟩ 
+              | Sum.inr (Normal.neu normN) => match progress M with
+                    | Sum.inl ⟨_ , s⟩ => Sum.inl  ⟨_ , Step.app2 s⟩ 
+                    | Sum.inr normM => Sum.inr (Normal.neu (Neutral.app normN normM))
+
+def eval {Γ} (fuel : Nat) (t1 : Term Γ)
+  : Option (Σ t2, ((MultiStep t1 t2) × (Normal t2))) :=
+  match fuel with
+  | zero => none
+  | Nat.succ fuel' => match progress t1 with
+    | Sum.inl ⟨t' , s⟩ => do 
+        let ⟨final , steps , nf⟩ <- eval fuel' t'
+        some ⟨final , MultiStep.step s steps , nf⟩
+    | Sum.inr norm => some ⟨t1 , MultiStep.halt , norm⟩
+
+-- infix:50 " ~>> " => MultiStep
+-- infix:50 " ~>> " => MultiStep
+
+def multiTrans {Γ} {L M N : Term Γ}
+  (s1 : MultiStep L M) (s2 : MultiStep M N) : MultiStep L N :=
+  match s1 with
+  | MultiStep.halt => s2
+  | MultiStep.step s steps => MultiStep.step s (multiTrans steps s2)
+
+def appLCong {Γ} {L L' M : Term Γ}
+  (m : MultiStep L L') : MultiStep (app L M) (app L' M) :=
+  match m with
+  | MultiStep.halt => MultiStep.halt
+  | MultiStep.step s steps => MultiStep.step (Step.app1 s) (appLCong steps)
+
+def appRCong {Γ} {L M M' : Term Γ}
+  (m : MultiStep M M') : MultiStep (app L M) (app L M') :=
+  match m with
+  | MultiStep.halt => MultiStep.halt
+  | MultiStep.step s steps => MultiStep.step (Step.app2 s) (appRCong steps)
+
+def appCong {n} {L L' M M' : Term n}
+  (m1 : MultiStep L L') (m2 : MultiStep M M') : MultiStep (app L M) (app L' M') :=
+  multiTrans (appLCong m1) (appRCong m2)
+
+def lamCong {Γ} {M M' : Term (succ Γ)}
+  (m : MultiStep M M') : MultiStep (lam M) (lam M') :=
+  match m with
+  | MultiStep.halt => MultiStep.halt
+  | MultiStep.step s steps => MultiStep.step (Step.lam s) (lamCong steps)
+
+--------------------------------------------------------------------------------
+---------- This section came from Subsitution.agda in plfa ---------------------
+--------------------------------------------------------------------------------
+
+-- The substitution alegra; all substitution can be built using these
+def ids {Γ} : Subst Γ Γ := var
+
+def shift {Γ} : Subst Γ (succ Γ) :=
+  fun x => var (Var.succ x)
+
+def cons {Γ Δ} (t : Term Δ) (sub : Subst Γ Δ) : Subst (succ Γ) Δ :=
+  fun x => match x with
+    | Var.zero => t
+    | Var.succ x' => sub x'
+
+def compose {n1 n2 n3} : Subst n1 n2 → Subst n2 n3 → Subst n1 n3 :=
+  fun sub1 sub2 => subst sub2 ∘ sub1
+
+def renToSub {Γ Δ} : Ren Γ Δ → Subst Γ Δ :=
+  fun ren => ids ∘ ren
+
+def bla : Nat → Nat := fun x => x 
+
+theorem subIdL {Γ Δ} {sub : Subst Γ Δ} : compose ids sub = sub :=
+  by apply funext
+     intro x
+     rfl
+     
+
+theorem subDist {n1 n2 n3} {sub1 : Subst n1 n2} {sub2 : Subst n2 n3} {M : Term n2}
+  : (compose (cons M sub1) sub2) = (cons (subst sub2 M) (compose sub1 sub2)) :=
+  by apply funext
+     intro x
+     cases x
+     . rfl
+     . rfl
+
+theorem renExt {n1 n2} {ren : Ren n1 n2} : renToSub (ext ren) = exts (renToSub ren) := by
+  apply funext
+  intro x
+  cases x
+  . rfl
+  . rfl
+
+
+theorem renameSubstRen {n1 n2} {ren : Ren n1 n2} {M : Term n1}
+  : rename ren M = subst (renToSub ren) M := by
+  cases M
+  . rfl
+  . simp [rename, subst, renExt]; rw [(Eq.symm renExt)]; apply renameSubstRen
+  . simp [subst, rename]
+    apply And.intro
+    . apply renameSubstRen
+    . apply renameSubstRen
+
+theorem extsConsShift {n1 n2} {sub : Subst n1 n2}
+  : exts sub = cons (var Var.zero) (compose sub shift) := by
+  apply funext
+  intros x
+  cases x
+  . rfl
+  . apply renameSubstRen
+
+theorem substZConsIds {Γ} {M : Term Γ} : substZero M = (cons M ids) := by
+  apply funext
+  intro x
+  cases x
+  . rfl
+  . rfl
+
+theorem extsIds {Γ} : exts ids = @ids (succ Γ) := by
+  apply funext
+  intro x
+  cases x
+  . rfl
+  . rfl
+
+theorem subId {Γ} {M : Term Γ} : subst ids M = M := by
+  induction M
+  . rfl
+  . simp [subst]
+    rw [extsIds]
+    assumption
+  . simp [subst]
+    apply And.intro
+    . assumption
+    . assumption
+
+theorem renameId {Γ} {M : Term Γ} : rename (fun x => x) M = M := by
+  rw [renameSubstRen]
+  apply subId
+
+theorem subIdR {Γ Δ} {sub : Subst Γ Δ} : (compose sub ids) = sub := by
+  apply funext
+  intro x
+  apply subId
+
+theorem composeExt {n1 n2 n3} {ren2 : Ren n2 n3} {ren1 : Ren n1 n2}
+  : (ext ren2) ∘ (ext ren1) = ext (ren2 ∘ ren1) := by
+  apply funext
+  intro x
+  cases x
+  . rfl
+  . rfl
+
+theorem composeRename {n1} {M : Term n1} 
+  : ∀ {n2 n3} {ren : Ren n2 n3} {ren' : Ren n1 n2},
+    rename ren (rename ren' M) = rename (ren ∘ ren') M := by
+  induction M with
+  | var x => intros; rfl
+  | lam t ih =>
+    intros n2 n3 ren ren'
+    simp [rename]
+    rw [← composeExt]
+    apply (@ih (succ n2) (succ n3) (ext ren) (ext ren'))
+  | app t1 t2 ih1 ih2 =>
+    intros
+    simp [rename]
+    apply And.intro
+    . apply ih1
+    . apply ih2
+
+-- This is a helper used in commuteSubstRename, but seemingly lean has problems if I put its definition in there with the let tactic.
+-- It seems that lean can't simp by locally defined definitions?
+def ren' {ren : {Γ : Context} → Ren Γ (Nat.succ Γ)}
+  : ∀{Γ}, Ren Γ (succ Γ) := fun {Γ} => match Γ with
+  | Nat.zero => fun y => False.rec (noVarZero y)
+  | Nat.succ x' => ext ren
+
+theorem commuteSubstRename {Γ} {M : Term Γ}
+  : ∀ {Δ} {sub : Subst Γ Δ}
+  {ren : ∀{Γ}, Ren Γ (succ Γ)},
+   (r : ∀{x : Var Γ}, exts sub (ren x) = rename ren (sub x))
+  → subst (exts sub) (rename ren M) = rename ren (subst sub M) := by
+  induction M with
+  | var x => intro Δ sub ren r; apply r
+  | lam t ih =>
+    intro Δ sub ren r
+    simp [subst, rename]
+    apply (@ih _ (exts sub) ren')
+    simp [ren']
+    intro x
+    cases x with
+    | zero => rfl
+    | succ y =>
+      simp [ext, exts]
+      simp [exts] at r
+      rw [r]
+      simp [composeRename]
+      rfl
+  | app t1 t2 ih1 ih2 =>
+    intro Δ sub ren r
+    simp [subst, rename]
+    apply And.intro
+    . apply (ih1 r)
+    . apply (ih2 r)
+
+theorem extsSeq {Γ Δ Δ'} {sub1 : Subst Γ Δ} {sub2 : Subst Δ Δ'}
+  : compose (exts sub1) (exts sub2) = exts (compose sub1 sub2) := by
+  apply funext
+  intro x
+  cases x with
+  | zero => rfl
+  | succ y =>
+    simp [compose]
+    simp [exts]
+    rw [<- commuteSubstRename]
+    . rfl
+    . intro x; rfl
+
+theorem subSub {n1} {M : Term n1}
+  : ∀ {n2 n3} {sub1 : Subst n1 n2} {sub2 : Subst n2 n3},
+  subst sub2 (subst sub1 M) = subst (compose sub1 sub2) M := by
+    induction M with
+    | var i => intros; rfl
+    | app t1 t2 ih1 ih2 =>
+        intros
+        simp [subst]
+        apply And.intro
+        apply ih1
+        apply ih2
+    | lam t ih =>
+        intros
+        --
+        simp [subst]
+        rw [ih]
+        rw [extsSeq]
+
+theorem renameSubst {Γ Δ Δ' : Context} {M : Term Γ} {ren : Ren Γ Δ} {sub : Subst Δ Δ'} 
+  : subst sub (rename ren M) = subst (sub ∘ ren) M := by
+  rw [renameSubstRen]
+  simp [subSub]
+  rfl
+
+def bloo {n : Nat} : Nat := n
+
+theorem subAssoc {n1 n2 n3 n4} {sub1 : Subst n1 n2} {sub2 : Subst n2 n3}
+  {sub3 : Subst n3 n4}
+  : compose (compose sub1 sub2) sub3 = compose sub1 (compose sub2 sub3) := by
+  -- 
+  apply funext
+  intro x
+  simp [compose]
+  apply subSub
+
+#check substZConsIds
+#check extsConsShift
+#check subDist
+#check subAssoc
+#check subIdR
+#check subIdL
+#check substZConsIds
+
+theorem subTail {n1 n2} {M : Term n2} {sub : Subst n1 n2}
+  : compose shift (cons M sub) = sub := by
+  apply funext
+  intros x
+  rfl
+
+-- probably don't need this?
+theorem renSuccShift {n}
+  : renToSub (Var.succ) = @shift n := by
+  -- apply funext
+  -- intro x
+  rfl
+
+theorem substCommute {n1 n2} {N : Term (succ n1)} {M : Term n1} {sub : Subst n1 n2}
+  : subLast (subst (exts sub) N) (subst sub M)
+    = subst sub (subLast N M) := by
+  simp [subLast]
+  -- rw [extsConsShift]
+  -- rw [substZConsIds]
+  -- rw [substZConsIds]
+  rw [subSub, subSub]
+  have p : (compose (exts sub) (substZero (subst sub M))) = (compose (substZero M) sub)
+    := by
+    rw [extsConsShift]
+    rw [substZConsIds]
+    rw [substZConsIds]
+    rw [subDist]
+    rw [subDist]
+    rw [subIdL]
+    rw [subAssoc]
+    rw [subTail]
+    rw [subIdR]
+    rfl
+  rw [p]
+
+theorem renameSubstCommute {Γ Δ} {N : Term (succ Γ)} {M : Term Γ} {ren : Ren Γ Δ}
+  : subLast (rename (ext ren) N) (rename ren M) = rename ren (subLast N M) := by
+  rw [renameSubstRen]
+  rw [renameSubstRen]
+  rw [renameSubstRen]
+  rw [renExt]
+  rw [substCommute]
+
+--------------------------------------------------------------------------------
+---------- This section came from Confluence.agda in plfa ----------------------
+--------------------------------------------------------------------------------
+-- I have heavily modified this section from PLFA
+
+def SubStep {n1 n2 : Context} (sub1 sub2 : Subst n1 n2) : Type :=
+  ∀ {x}, Step (sub1 x) (sub2 x)
+
+def MultiSubStep {n1 n2} (sub1 sub2 : Subst n1 n2) : Type :=
+  ∀ {x}, MultiStep (sub1 x) (sub2 x)
+
+def singletonStep {n} {t1 t2 : Term n} (step : Step t1 t2)
+  : MultiStep t1 t2 := MultiStep.step step MultiStep.halt
+
+theorem multiSubStepHalt {n1 n2} {sub : Subst n1 n2} : MultiSubStep sub sub := by
+  intro x
+  apply MultiStep.halt
+
+theorem multiSubStepStep {n1 n2} {sub1 sub2 sub3 : Subst n1 n2}
+  (step : SubStep sub1 sub2) (mstep : MultiSubStep sub2 sub3)
+  : MultiSubStep sub1 sub3 := by
+  intro x
+  apply MultiStep.step step mstep
+
+theorem renameStep {n1}
+  {t1 t2 : Term n1} (step : Step t1 t2)
+  : ∀ {n2} {ren : Ren n1 n2},
+    Step (rename ren t1) (rename ren t2) := by 
+  induction step with
+  -- . simp [rename]; apply Step.app1;  
+  | app1 _ ih => intros; simp [rename]; apply Step.app1; apply ih
+  | app2 _ ih => intros; simp [rename]; apply Step.app2; apply ih
+  | lam _ ih => intros; simp [rename]; apply Step.lam; apply ih
+  | beta =>
+    intros
+    simp [rename]
+    rw [<- renameSubstCommute]
+    apply Step.beta
+  | eta =>
+    intros
+    simp [rename]
+    rw [composeRename]
+    -- TODO: decide if this lemma should be defined outside. Is it needed elsewhere?
+    have renExtLemma : ∀{n1 n2} {ren : Ren n1 n2}, ext ren ∘ Var.succ = Var.succ ∘ ren := by
+      intros
+      apply funext
+      intro x
+      simp [Function.comp]
+      simp [ext]
+    rw [renExtLemma]
+    rw [<- composeRename]
+    apply Step.eta
+
+theorem renameMultiStep {n1}
+  {t1 t2 : Term n1} {mstep : MultiStep t1 t2}
+  : ∀ {n2} {ren : Ren n1 n2},
+    MultiStep (rename ren t1) (rename ren t2) := by 
+  induction mstep with
+  | halt => intros; apply MultiStep.halt
+  | step s _ms ih =>
+    intros
+    apply MultiStep.step
+    apply (renameStep s)
+    apply ih
+  
+
+theorem subStepExts {n1 n2} {sub1 sub2 : Subst n1 n2}
+  : SubStep sub1 sub2 → MultiSubStep (exts sub1) (exts sub2) := by 
+  intro step x
+  cases x with
+  | zero => simp [exts]; apply MultiStep.halt
+  | succ y => simp [exts]; apply renameMultiStep; apply singletonStep; apply step
+
+theorem subMultiStepExts {n1 n2} {sub1 sub2 : Subst n1 n2}
+  : MultiSubStep sub1 sub2 → MultiSubStep (exts sub1) (exts sub2) := by 
+  intro mstep x
+  cases x with
+  | zero => simp [exts]; apply multiSubStepHalt
+  | succ y =>
+    simp [exts]
+    apply renameMultiStep
+    apply mstep
+
+
+theorem substStep {n1}
+  {t1 t2 : Term n1} (step : Step t1 t2)
+  : ∀ {n2} {sub : Subst n1 n2},
+    Step (subst sub t1) (subst sub t2) := by 
+  induction step with
+  | app1 _ ih => intros; simp [subst]; apply Step.app1; apply ih
+  | app2 _ ih => intros; simp [subst]; apply Step.app2; apply ih
+  | lam _ ih => intros; simp [subst]; apply Step.lam; apply ih
+  | beta =>
+    intros
+    simp [subst]
+    rw [<- substCommute]
+    apply Step.beta
+  | @eta _ N =>
+    intros n2 sub
+    simp [subst]
+    have lemma : subst (exts sub) (rename Var.succ N) = rename Var.succ (subst sub N) := by
+      rw [renameSubstRen]
+      rw [renameSubstRen]
+      rw [subSub]
+      rw [subSub]
+      rw [renSuccShift]
+      rw [renSuccShift]
+      rw [extsConsShift]
+      rw [subTail]
+    rw [lemma]
+    apply Step.eta
+
+theorem substMultiStep {n1}
+  {t1 t2 : Term n1} (step : MultiStep t1 t2)
+  {n2} {sub : Subst n1 n2}
+  : MultiStep (subst sub t1) (subst sub t2) := by 
+  induction step with
+  | halt => apply MultiStep.halt
+  | step s ms ih =>
+    apply MultiStep.step
+    apply (substStep s)
+    apply ih
+  
+  
+theorem stepSubs {n1} {t : Term n1} :
+   ∀ {n2} {sub1 sub2 : Subst n1 n2} {_sstep : MultiSubStep sub1 sub2},
+    MultiStep (subst sub1 t) (subst sub2 t) := by
+  induction t with
+  | var x => intro n2 sub1 sub2 sstep; apply sstep
+  | app t1 t2 ih1 ih2 =>
+    intro n2 sub1 sub2 sstep
+    simp [subst]
+    apply appCong
+    apply ih1; apply sstep
+    apply ih2; apply sstep
+  | lam t ih =>
+    intro n2 sub1 sub2 sstep
+    simp [subst]
+    apply lamCong
+    apply ih
+    apply subMultiStepExts
+    apply sstep
+  
+theorem parSubstZero {Γ} {M M' : Term Γ}
+   {mstep: MultiStep M M' }
+   : MultiSubStep (substZero M) (substZero M') := by
+   intro x
+   cases x
+   . apply mstep
+   . simp [substZero]
+     apply MultiStep.halt
+
+theorem stepSub {Γ} {N N' : Term (succ Γ)} {M M' : Term Γ}
+  (stepN : MultiStep N N') (stepM : MultiStep M M')
+  : MultiStep (subLast N M) (subLast N' M') := by
+  simp [subLast]
+  let lemma : MultiStep (subst (substZero M) N) (subst (substZero M) N') := by
+      apply substMultiStep
+      apply stepN
+  apply (multiTrans lemma)
+  apply stepSubs
+  apply parSubstZero
+  apply stepM
+
+def superStep {Γ} (t : Term Γ) : Term Γ :=
+  match t with
+  | var x => var x
+  | app (lam t1) t2 => subLast (superStep t1) (superStep t2)
+  | app t1 t2 => app (superStep t1) (superStep t2)
+  | lam t => lam (superStep t)
+
+inductive BetaStep : ∀{Γ}, Term Γ → Term Γ → Type where  
+| app1 : ∀ {Γ} {L L' M : Term Γ},
+    BetaStep L L'
+    → BetaStep (app L M) (app L' M)
+| app2 : ∀ {Γ} {L M M' : Term Γ},
+    BetaStep M M'
+    → BetaStep (app L M) (app L M')
+| beta : ∀ {Γ} {N : Term (succ Γ)} {M : Term Γ},
+    BetaStep (app (lam N) M) (subLast N M)
+| lam : ∀ {Γ} {N N' : Term (succ Γ)},
+    BetaStep N N' → BetaStep (lam N) (lam N')
+
+inductive EtaStep : ∀{Γ}, Term Γ → Term Γ → Type where  
+| eta : ∀{Γ} {N : Term Γ},
+    EtaStep N (lam (app (rename Var.succ N) (var Var.zero)))
+
+theorem selfSuperStep {Γ} {t : Term Γ}
+  : MultiStep t (superStep t) :=
+  match t with
+  | var i => by simp [superStep]; apply MultiStep.halt
+  | app (lam t1) t2 => by
+    simp [superStep]
+    apply MultiStep.step
+    apply Step.beta
+    apply stepSub
+    apply selfSuperStep
+    apply selfSuperStep
+  | app (app t1 t2) t3 => by
+    simp [superStep]
+    apply appCong
+    apply selfSuperStep
+    apply selfSuperStep
+  | app (var i) t2 => by
+    simp [superStep]
+    apply appCong
+    apply MultiStep.halt
+    apply selfSuperStep
+    --
+  | lam t => by
+    simp [superStep]
+    apply lamCong
+    apply selfSuperStep
+
+theorem triangleProperty {Γ} {t t' : Term Γ}
+  {step : BetaStep t t'}
+  : MultiStep t' (superStep t) :=
+  match t, t', step with
+  | .(_), .(_), BetaStep.lam s => by
+    simp [superStep]
+    apply lamCong
+    apply triangleProperty
+    apply s
+  | (app (var i) t2), .(_), BetaStep.app2 s => by
+    simp [superStep]
+    apply appRCong
+    apply triangleProperty
+    apply s
+  | (app (lam t1) t2), .(_), BetaStep.app2 s => by
+    simp [superStep]
+    apply MultiStep.step
+    apply Step.beta
+    apply stepSub
+    apply selfSuperStep
+    apply triangleProperty; apply s
+  | (app (app t1 t2) t3), .(_), BetaStep.app2 s => by
+    simp [superStep]
+    apply appCong
+    apply selfSuperStep
+    apply triangleProperty; apply s
+  | .(_), .(_), BetaStep.beta => by
+    simp [superStep]
+    apply stepSub
+    apply selfSuperStep
+    apply selfSuperStep
+  | (app (lam t1) t2), .(_), BetaStep.app1 (BetaStep.lam s) => by
+    simp [superStep]
+    apply MultiStep.step
+    apply Step.beta
+    apply stepSub
+    apply triangleProperty; apply s
+    apply selfSuperStep
+  | (app (app t1 t2) t3), .(_), BetaStep.app1 s => by
+    simp [superStep]
+    apply appCong
+    apply triangleProperty; apply s
+    apply selfSuperStep
+
+theorem betaToStep {n} {t1 t2 : Term n}
+  {bstep : BetaStep t1 t2} : Step t1 t2 := by
+  induction bstep with
+  | app1 _ ih => apply Step.app1; apply ih
+  | app2 _ ih => apply Step.app2; apply ih
+  | lam _ ih => apply Step.lam; apply ih
+  | beta => apply Step.beta
+
+-- theorem stepToBeta {n} {t1 t2 : Term n}
+--   {step : Step t1 t2}
+--   : BetaStep t1 t2 ⊕ EtaStep t1 t2 := by
+--   induction step with
+--   | app1 _ ih => apply Sum.inl; apply BetaStep.app1; apply ih
+--   | app2 _ ih => apply Sum.inl; apply BetaStep.app2; apply ih
+--   | lam _ ih => apply Sum.inl; apply BetaStep.lam; apply ih
+--   | beta => apply Sum.inl; apply BetaStep.beta
+--   | eta => apply Sum.inr; apply EtaStep.eta
+
+theorem subWeaken {n} {M N : Term n}
+  : subLast (rename Var.succ M) N = M := by
+  simp [subLast]
+  rw [renameSubstRen]
+  rw [subSub]
+  have lemma: compose (renToSub Var.succ) (substZero N) = ids := by
+    apply funext
+    intro x
+    cases x
+    . rfl
+    . rfl
+  rw [lemma]
+  apply subId
+
+theorem betaEtaCaseLemma {Γ} {M : Term Γ} {N : Term (succ Γ)}
+  : MultiStep (app (lam (app (rename Var.succ (lam N)) (var Var.zero))) M) (subLast N M)
+  := by
+     apply MultiStep.step
+     apply Step.beta
+     have lemma {n} {a : Term (succ n)} {M : Term n}
+       : subLast (app (rename Var.succ (lam a)) (var Var.zero)) M
+       = app (lam a) M := by
+       have lemma2 {n} {a : Term (succ n)} {M : Term n} 
+         : subLast (app (rename Var.succ (lam a)) (var Var.zero)) M
+           = app (subLast (rename Var.succ (lam a)) M) M := by
+           simp [subLast, subst, substZero]
+       rw [lemma2]
+       rw [subWeaken]
+     rw [lemma]
+     apply MultiStep.step
+     apply Step.beta
+     apply MultiStep.halt
+
+theorem singleStepConfluence {Γ} {t t1 t2 : Term Γ}
+  (step1 : Step t t1) (step2 : Step t t2)
+  : Σ t', MultiStep t1 t' × MultiStep t2 t' :=
+  match step1, step2 with
+  | Step.lam a, Step.lam b => match singleStepConfluence a b with
+    | ⟨t, m1, m2⟩ => ⟨lam t, lamCong m1, lamCong m2⟩
+  | Step.app1 a, Step.app1 b => match singleStepConfluence a b with
+    | ⟨_, m1, m2⟩ => ⟨_, appLCong m1, appLCong m2⟩
+  | Step.app2 a, Step.app2 b => match singleStepConfluence a b with
+    | ⟨_, m1, m2⟩ => ⟨_, appRCong m1, appRCong m2⟩
+  | Step.app2 a, Step.app1 b => 
+    ⟨_, singletonStep (Step.app1 b), singletonStep (Step.app2 a)⟩
+  | Step.app1 a, Step.app2 b =>
+    ⟨_, singletonStep (Step.app2 b), singletonStep (Step.app1 a)⟩
+  | Step.eta, x => ⟨_,
+        singletonStep (Step.lam (Step.app1 (renameStep x)))
+        , singletonStep Step.eta⟩
+  | x, Step.eta => ⟨_,
+        singletonStep Step.eta
+        , singletonStep (Step.lam (Step.app1 (renameStep x)))⟩ 
+  | Step.beta, Step.beta => ⟨_, MultiStep.halt, MultiStep.halt⟩
+  | Step.beta, Step.app1 (Step.lam s) => ⟨_, stepSub (singletonStep s) MultiStep.halt,
+    singletonStep Step.beta⟩
+  | Step.beta, Step.app1 (Step.eta) => ⟨_, MultiStep.halt, betaEtaCaseLemma⟩
+  | Step.beta, Step.app2 a =>
+    ⟨_, stepSub MultiStep.halt (singletonStep a), singletonStep Step.beta⟩ 
+  | Step.app2 a, Step.beta =>
+    ⟨_, singletonStep Step.beta, stepSub MultiStep.halt (singletonStep a)⟩ 
+  | Step.app1 (Step.lam s), Step.beta => ⟨_, singletonStep Step.beta,
+    stepSub (singletonStep s) MultiStep.halt⟩
+  | Step.app1 Step.eta, Step.beta => ⟨_, betaEtaCaseLemma, MultiStep.halt⟩
+
+theorem strip {Γ} {t t1 t2 : Term Γ}
+  (step1 : Step t t1) (mstep2 : MultiStep t t2)
+  : Σ t', MultiStep t1 t' × MultiStep t2 t' :=
+  match mstep2 with
+  | MultiStep.halt => ⟨_, MultiStep.halt, singletonStep step1⟩
+  | MultiStep.step s ms =>
+    let bla := singleStepConfluence step1 s
+    match strip step1 mstep2 with
+    | ⟨t', ms1, ms2⟩ => ⟨_, _⟩
+
+-- theorem confluence {Γ} {t t1 t2 : Term Γ}
+--   (mstep1 : MultiStep t t1) (mstep2 : MultiStep t t2)
+--   : Σ t', MultiStep t1 t' × MultiStep t2 t' := by
+--   induction mstep1 with
+--   | halt => exact ⟨_, mstep2, MultiStep.halt⟩
+--   | step s1 ms1 ih1 => induction mstep2 with
+--             | halt => exact ⟨_, MultiStep.halt, MultiStep.step s1 ms1⟩
+--             | step s2 ms2 ih2 => sorry
+
+
+-- TODO: follow this proof https://doi.org/10.1006/inco.1995.1057
+
+/- 
+Something that we will need
+Equivalence relation on terms R
+
+lamR : R t1 t2 → R (lam t1) (lam t2)
+appR : R a1 a2 → R b1 b2 → R (app a1 b1) (app a2 b2)
+
+prove using *cong
+---/
+
+
+-- Something that is slightly concerning is if the use of funext and/or quotients
+-- will make things non-computational in a way what will cause problems.
+-- I need to think this through carefully.
+
+-- I believe that the following demonstrates that quotients don't actually
+-- get in the way of computation in lean:
+
+def Bla := @Quot Nat (fun x y => x = y)
+
+def getNat : Bla → Nat :=
+  Quot.lift (fun x => x) (by
+    intros a b p
+    simp
+    assumption
+  )
+
+theorem canICompute : (getNat (Quot.mk (fun x y => x = y) 5)) = 5 := by
+  simp
+
+-- Some other very strange reduction behaviour that I noticed: any type with
+-- only one constructor won't block reduction, but if you uncomment
+-- the second constructor, then it does block reduction.
+
+inductive MyUnit : Type 
+| myunit : MyUnit
+-- | myunit2 : MyUnit
+
+def test3 : MyUnit → Nat → Nat := fun p n =>
+  match p with
+  | MyUnit.myunit => n * n + 2
+  -- | MyUnit.myunit2 => n * n + 2
+
+axiom typeAxiom : MyUnit
+
+theorem canICompute2 : test3 typeAxiom 2 = 6 := by
+  simp [test3]
+  --
